examples/compute/src/theory/bir_computeScript.sml
@@ -193,7 +193,7 @@ Theorem bir_eval_unaryexp_eq_compute_unaryexp:
 Proof
   Cases_on `unaryexp` >>
   Cases_on `v1` >> Cases_on `v` >>
-  rw [bir_eval_unaryexp_def, bir_compute_unaryexp_def] >>
+  rw [bir_eval_unaryexp_cases, bir_compute_unaryexp_def] >>
   rw [bir_eval_unaryexp_imm_cases, bir_compute_unaryexp_imm_def] >>
   Cases_on `b` >> Cases_on `b'` >>
   rw [bir_compute_unaryexp_imm_def, fetch "bir" "bir_imm_t_nchotomy", bir_unaryexp_get_oper_def] >>
